Tweaked the relation a bit in order to be able to prove completeness w.r.t. contextual approximation

theories/L6_PCPS/List_util.v
@@ -1,61 +1,128 @@
-Require Import Coq.Lists.List Coq.Relations.Relations Coq.Classes.RelationClasses.
+Require Import Coq.Lists.List Coq.Relations.Relations Coq.Classes.RelationClasses
+        Coq.omega.Omega.
 Import ListNotations.
 
 Ltac inv H := inversion H; clear H; subst.
 
+(** Asymmetric version of Forall2 *) 
+Inductive Forall2_asym {A} (R : relation A) : list A -> list A -> Prop :=
+| Forall2_asym_nil : forall l, Forall2_asym R [] l
+| Forall2_asym_cons :
+    forall x y l l', R x y -> Forall2_asym R l l' -> Forall2_asym R (x :: l) (y :: l').
+
+Hint Constructors Forall2_asym.
+
 Lemma Forall2_length {A} (R : A -> A -> Prop) (l1 l2 : list A) :
-    Forall2 R l1 l2 -> length l1 = length l2. 
-  Proof.
-    revert l2. induction l1 as [| x xs IHxs ]; intros l2 H.
-    - inv H; eauto.
-    - inv H. simpl. f_equal. eauto.
-  Qed.
+  Forall2 R l1 l2 -> length l1 = length l2. 
+Proof.
+  revert l2. induction l1 as [| x xs IHxs ]; intros l2 H.
+  - inv H; eauto.
+  - inv H. simpl. f_equal. eauto.
+Qed.
 
-  Lemma Forall2_monotonic {A} (R R' : A -> A -> Prop) (l1 l2 : list A) :
-    (forall x1 x2, R x1 x2 -> R' x1 x2) ->
-    Forall2 R l1 l2 ->
-    Forall2 R' l1 l2.
-  Proof.
-    intros H. revert l2.
-    induction l1 as [| x xs IHxs ]; intros l2 Hall.
-    - inv Hall; eauto. 
-    - destruct l2; inv Hall. constructor; eauto.
-  Qed.
+Lemma Forall2_asym_length {A} (R : A -> A -> Prop) (l1 l2 : list A) :
+  Forall2_asym R l1 l2 -> length l1 <= length l2. 
+Proof.
+  revert l2. induction l1 as [| x xs IHxs ]; intros l2 H.
+  - inv H; simpl. omega.
+  - inv H. simpl. eapply IHxs in H4. omega.
+Qed.
 
-  Lemma Forall2_refl {A} (R : A -> A -> Prop) (l : list A) :
-    Reflexive R ->
-    Forall2 R l l.
-  Proof.
-    intros H. induction l as [| x l IHl]; eauto.
-  Qed.
-  
-  Lemma Forall2_trans {A} (R : A -> A -> Prop) (l1 l2 l3 : list A) :
-    Transitive R ->
-    Forall2 R l1 l2 ->
-    Forall2 R l2 l3 ->
-    Forall2 R l1 l3.
-  Proof.
-    intros Htrans.
-    revert l2 l3. induction l1 as [| x l IHl ]; intros l2 l3 H1 H2.
-    - inv H1. inv H2. constructor.
-    - inv H1. inv H2. constructor; eauto.
-  Qed.      
+Lemma Forall2_monotonic {A} (R R' : A -> A -> Prop) (l1 l2 : list A) :
+  (forall x1 x2, R x1 x2 -> R' x1 x2) ->
+  Forall2 R l1 l2 ->
+  Forall2 R' l1 l2.
+Proof.
+  intros H. revert l2.
+  induction l1 as [| x xs IHxs ]; intros l2 Hall.
+  - inv Hall; eauto. 
+  - destruct l2; inv Hall. constructor; eauto.
+Qed.
 
-  Lemma Forall2_trivial {A} (R : A -> A -> Prop) (l1 l2 : list A) :
-    (forall x y, R x y) ->
-    (length l1 = length l2) -> 
-    Forall2 R l1 l2.
-  Proof.
-    intros H.
-    revert l2; induction l1 as [| x l IHl]; intros l2 Hlen;
-    destruct l2; try discriminate; eauto.
-  Qed.
+Lemma Forall2_asym_monotonic {A} (R R' : A -> A -> Prop) (l1 l2 : list A) :
+  (forall x1 x2, R x1 x2 -> R' x1 x2) ->
+  Forall2_asym R l1 l2 ->
+  Forall2_asym R' l1 l2.
+Proof.
+  intros H. revert l2.
+  induction l1 as [| x xs IHxs ]; intros l2 Hall.
+  - inv Hall; eauto. 
+  - destruct l2; inv Hall. constructor; eauto.
+Qed.
 
-  Lemma Forall2_same {A} (R : A -> A -> Prop) l:
-    (forall x, List.In x l -> R x x) ->
-    Forall2 R l l.
-  Proof.
-    induction l; intros H; constructor.
-    - apply H. constructor; eauto.
-    - apply IHl. intros. apply H. constructor 2; eauto.
-  Qed.
+Lemma Forall2_refl {A} (R : A -> A -> Prop) (l : list A) :
+  Reflexive R ->
+  Forall2 R l l.
+Proof.
+  intros H. induction l as [| x l IHl]; eauto.
+Qed.
+
+Lemma Forall2_asym_refl {A} (R : A -> A -> Prop) (l : list A) :
+  Reflexive R ->
+  Forall2_asym R l l.
+Proof.
+  intros H. induction l as [| x l IHl]; eauto.
+Qed.
+
+Lemma Forall2_trans {A} (R : A -> A -> Prop) (l1 l2 l3 : list A) :
+  Transitive R ->
+  Forall2 R l1 l2 ->
+  Forall2 R l2 l3 ->
+  Forall2 R l1 l3.
+Proof.
+  intros Htrans.
+  revert l2 l3. induction l1 as [| x l IHl ]; intros l2 l3 H1 H2.
+  - inv H1. inv H2. constructor.
+  - inv H1. inv H2. constructor; eauto.
+Qed.      
+
+Lemma Forall2_asym_trans {A} (R : A -> A -> Prop) (l1 l2 l3 : list A) :
+  Transitive R ->
+  Forall2_asym R l1 l2 ->
+  Forall2_asym R l2 l3 ->
+  Forall2_asym R l1 l3.
+Proof.
+  intros Htrans.
+  revert l2 l3. induction l1 as [| x l IHl ]; intros l2 l3 H1 H2.
+  - inv H1. inv H2; eauto.
+  - inv H1. inv H2; eauto.
+Qed.      
+
+Lemma Forall2_trivial {A} (R : A -> A -> Prop) (l1 l2 : list A) :
+  (forall x y, R x y) ->
+  (length l1 = length l2) -> 
+  Forall2 R l1 l2.
+Proof.
+  intros H.
+  revert l2; induction l1 as [| x l IHl]; intros l2 Hlen;
+  destruct l2; try discriminate; eauto.
+Qed.
+
+Lemma Forall2_asym_trivial {A} (R : A -> A -> Prop) (l1 l2 : list A) :
+  (forall x y, R x y) ->
+  (length l1 <= length l2) -> 
+  Forall2_asym R l1 l2.
+Proof.
+  intros H.
+  revert l2; induction l1 as [| x l IHl]; intros l2 Hlen; eauto.
+  destruct l2; simpl in *; try omega. constructor; eauto.
+  eapply IHl; omega.
+Qed.
+
+Lemma Forall2_same {A} (R : A -> A -> Prop) l:
+  (forall x, List.In x l -> R x x) ->
+  Forall2 R l l.
+Proof.
+  induction l; intros H; constructor.
+  - apply H. constructor; eauto.
+  - apply IHl. intros. apply H. constructor 2; eauto.
+Qed.
+
+Lemma Forall2_asym_same {A} (R : A -> A -> Prop) l:
+  (forall x, List.In x l -> R x x) ->
+  Forall2_asym R l l.
+Proof.
+  induction l; intros H; constructor.
+  - apply H. constructor; eauto.
+  - apply IHl. intros. apply H. constructor 2; eauto.
+Qed.
